protocol-tests/src/invariants/bridge_phase_monotonicity.rs
@@ -17,7 +17,9 @@
 //! is a prefix of one of the two legal sequences.
 
 use crate::Invariant;
-use dregg_cell::note_bridge::{BridgePhase, BridgeReceiptEnvelope};
+use dregg_cell::note_bridge::{
+    BridgePhase, BridgePhaseLog, BridgeReceiptEnvelope, compute_bridge_id,
+};
 use proptest::prelude::*;
 
 pub struct BridgePhaseMonotonicity;
